Start n-ary sums

theories/multiparty/langdef.v
@@ -7,41 +7,44 @@ Definition participant := nat.
 Definition endpoint := (session * participant)%type.
 
 Inductive val :=
-    | UnitV : val
-    | NatV : nat -> val
-    | PairV : val -> val -> val
-    | InjV : bool -> val -> val
-    | FunV : string -> expr -> val
-    | UFunV : string -> expr -> val
-    | ChanV : endpoint -> val
+  | UnitV : val
+  | NatV : nat -> val
+  | PairV : val -> val -> val
+  | InjV : bool -> val -> val
+  | InjNV : nat -> val -> val
+  | FunV : string -> expr -> val
+  | UFunV : string -> expr -> val
+  | ChanV : endpoint -> val
 
 with expr :=
-    | Val : val -> expr
-    | Var : string -> expr
-    | Pair : expr -> expr -> expr
-    | Inj : bool -> expr -> expr
-    | App : expr -> expr -> expr
-    | UApp : expr -> expr -> expr
-    | Lam : string -> expr -> expr
-    | ULam : string -> expr -> expr
-    | Send : participant -> expr -> expr -> expr
-    | Recv : participant -> expr -> expr
-    | Let : string -> expr -> expr -> expr
-    | LetUnit : expr -> expr -> expr
-    | LetProd : string -> string -> expr -> expr -> expr
-    | MatchVoid : expr -> expr
-    | MatchSum : expr -> string -> expr -> expr -> expr
-    | If : expr -> expr -> expr -> expr
-    | Spawn n : (fin n -> expr) -> expr
-    | Close : expr -> expr.
+  | Val : val -> expr
+  | Var : string -> expr
+  | Pair : expr -> expr -> expr
+  | Inj : bool -> expr -> expr
+  | InjN : nat -> expr -> expr
+  | App : expr -> expr -> expr
+  | UApp : expr -> expr -> expr
+  | Lam : string -> expr -> expr
+  | ULam : string -> expr -> expr
+  | Send : participant -> expr -> expr -> expr
+  | Recv : participant -> expr -> expr
+  | Let : string -> expr -> expr -> expr
+  | LetUnit : expr -> expr -> expr
+  | LetProd : string -> string -> expr -> expr -> expr
+  | MatchVoid : expr -> expr
+  | MatchSum : expr -> string -> expr -> expr -> expr
+  | MatchSumN n : expr -> (fin n -> expr) -> expr
+  | If : expr -> expr -> expr -> expr
+  | Spawn n : (fin n -> expr) -> expr
+  | Close : expr -> expr.
 
 Canonical Structure valO := leibnizO val.
 Canonical Structure exprO := leibnizO expr.
 
 CoInductive session_type' (T : Type) :=
-    | SendT : participant -> T -> session_type' T -> session_type' T
-    | RecvT : participant -> T -> session_type' T -> session_type' T
-    | EndT : session_type' T.
+  | SendT : participant -> T -> session_type' T -> session_type' T
+  | RecvT : participant -> T -> session_type' T -> session_type' T
+  | EndT : session_type' T.
 Arguments SendT {_} _ _ _.
 Arguments RecvT {_} _ _ _.
 Arguments EndT {_}.
@@ -49,36 +52,36 @@ Instance sendt_params : Params (@SendT) 1 := {}.
 Instance recvt_params : Params (@RecvT) 1 := {}.
 
 CoInductive session_type_equiv `{Equiv T} : Equiv (session_type' T) :=
-    | cteq_EndT : EndT ≡ EndT
-    | cteq_SendT t1 t2 s1 s2 p : t1 ≡ t2 -> s1 ≡ s2 -> SendT p t1 s1 ≡ SendT p t2 s2
-    | cteq_RecvT t1 t2 s1 s2 p : t1 ≡ t2 -> s1 ≡ s2 -> RecvT p t1 s1 ≡ RecvT p t2 s2.
+  | cteq_EndT : EndT ≡ EndT
+  | cteq_SendT t1 t2 s1 s2 p : t1 ≡ t2 -> s1 ≡ s2 -> SendT p t1 s1 ≡ SendT p t2 s2
+  | cteq_RecvT t1 t2 s1 s2 p : t1 ≡ t2 -> s1 ≡ s2 -> RecvT p t1 s1 ≡ RecvT p t2 s2.
 Existing Instance session_type_equiv.
 
 Lemma session_type_reflexive `{Equiv T} :
-    Reflexive (≡@{T}) -> Reflexive (≡@{session_type' T}).
+  Reflexive (≡@{T}) -> Reflexive (≡@{session_type' T}).
 Proof.
-    intros ?. cofix IH. intros []; constructor; done.
+  intros ?. cofix IH. intros []; constructor; done.
 Defined.
 
 Lemma session_type_symmetric `{Equiv T} :
-    Symmetric (≡@{T}) -> Symmetric (≡@{session_type' T}).
+  Symmetric (≡@{T}) -> Symmetric (≡@{session_type' T}).
 Proof.
-    intros ?. cofix IH. intros ??[]; constructor; done.
+  intros ?. cofix IH. intros ??[]; constructor; done.
 Defined.
 
 Lemma session_type_transitive `{Equiv T} :
-    Transitive (≡@{T}) -> Transitive (≡@{session_type' T}).
+  Transitive (≡@{T}) -> Transitive (≡@{session_type' T}).
 Proof.
-    intros ?. cofix IH. intros ???[]; inversion_clear 1; constructor; by etrans.
+  intros ?. cofix IH. intros ???[]; inversion_clear 1; constructor; by etrans.
 Defined.
 
 Global Instance session_type_equivalence `{Equiv T} :
-    Equivalence (≡@{T}) -> Equivalence (≡@{session_type' T}).
+  Equivalence (≡@{T}) -> Equivalence (≡@{session_type' T}).
 Proof.
-    split.
-    - apply session_type_reflexive. apply _.
-    - apply session_type_symmetric. apply _.
-    - apply session_type_transitive. apply _.
+  split.
+  - apply session_type_reflexive. apply _.
+  - apply session_type_symmetric. apply _.
+  - apply session_type_transitive. apply _.
 Qed.
 
 Global Instance sendt_proper `{Equiv T} p : Proper ((≡) ==> (≡) ==> (≡)) (@SendT T p).
@@ -87,80 +90,86 @@ Global Instance recvt_proper `{Equiv T} p : Proper ((≡) ==> (≡) ==> (≡)) (
 Proof. by constructor. Qed.
 
 Definition session_type_id {T} (s : session_type' T) : session_type' T :=
-    match s with
-    | SendT p t s' => SendT p t s'
-    | RecvT p t s' => RecvT p t s'
-    | EndT => EndT
-    end.
+  match s with
+  | SendT p t s' => SendT p t s'
+  | RecvT p t s' => RecvT p t s'
+  | EndT => EndT
+  end.
 
 Lemma session_type_id_id {T} (s : session_type' T) :
-    session_type_id s = s.
+  session_type_id s = s.
 Proof.
-    by destruct s.
+  by destruct s.
 Qed.
 
 Lemma session_type_equiv_alt `{Equiv T} (s1 s2 : session_type' T) :
-    session_type_id s1 ≡ session_type_id s2 -> s1 ≡ s2.
+  session_type_id s1 ≡ session_type_id s2 -> s1 ≡ s2.
 Proof.
-    intros.
-    rewrite -(session_type_id_id s1).
-    rewrite -(session_type_id_id s2).
-    done.
+  intros.
+  rewrite -(session_type_id_id s1).
+  rewrite -(session_type_id_id s2).
+  done.
 Defined.
 
 Lemma session_type_equiv_end_eq `{Equiv T} (s : session_type' T) :
-    s ≡ EndT -> s = EndT.
+  s ≡ EndT -> s = EndT.
 Proof.
-    by inversion 1.
+  by inversion 1.
 Qed.
 
 Canonical Structure session_type'O (T:ofe) := discreteO (session_type' T).
 
 CoInductive type :=
-    | UnitT : type
-    | VoidT : type
-    | NatT : type
-    | PairT : type -> type -> type
-    | SumT : type -> type -> type
-    | FunT : type -> type -> type
-    | UFunT : type -> type -> type
-    | ChanT : session_type' type -> type.
+  | UnitT : type
+  | VoidT : type
+  | NatT : type
+  | PairT : type -> type -> type
+  | SumT : type -> type -> type
+  | SumNT n : (fin n -> type) -> type
+  | FunT : type -> type -> type
+  | UFunT : type -> type -> type
+  | ChanT : session_type' type -> type.
 
 Definition type_id (t : type) :=
-    match t with
-    | UnitT => UnitT
-    | VoidT => VoidT
-    | NatT => NatT
-    | PairT t1 t2 => PairT t1 t2
-    | SumT t1 t2 => SumT t1 t2
-    | FunT t1 t2 => FunT t1 t2
-    | UFunT t1 t2 => UFunT t1 t2
-    | ChanT s => ChanT s
-    end.
+  match t with
+  | UnitT => UnitT
+  | VoidT => VoidT
+  | NatT => NatT
+  | PairT t1 t2 => PairT t1 t2
+  | SumT t1 t2 => SumT t1 t2
+  | SumNT n f => SumNT n f
+  | FunT t1 t2 => FunT t1 t2
+  | UFunT t1 t2 => UFunT t1 t2
+  | ChanT s => ChanT s
+  end.
 
 Lemma type_id_id t : type_id t = t.
 Proof.
-    by destruct t.
+  by destruct t.
 Qed.
 
 CoInductive type_equiv : Equiv type :=
-    | teq_UnitT : UnitT ≡ UnitT
-    | teq_VoidT : VoidT ≡ VoidT
-    | teq_NatT : NatT ≡ NatT
-    | teq_PairT t1 t2 t1' t2' : t1 ≡ t2 -> t1' ≡ t2' -> PairT t1 t1' ≡ PairT t2 t2'
-    | teq_SumT t1 t2 t1' t2' : t1 ≡ t2 -> t1' ≡ t2' -> SumT t1 t1' ≡ SumT t2 t2'
-    | teq_FunT t1 t2 t1' t2' : t1 ≡ t2 -> t1' ≡ t2' -> FunT t1 t1' ≡ FunT t2 t2'
-    | teq_UFunT t1 t2 t1' t2' : t1 ≡ t2 -> t1' ≡ t2' -> UFunT t1 t1' ≡ UFunT t2 t2'
-    | teq_ChanT s1 s2 : s1 ≡ s2 -> ChanT s1 ≡ ChanT s2.
+  | teq_UnitT : UnitT ≡ UnitT
+  | teq_VoidT : VoidT ≡ VoidT
+  | teq_NatT : NatT ≡ NatT
+  | teq_PairT t1 t2 t1' t2' : t1 ≡ t2 -> t1' ≡ t2' -> PairT t1 t1' ≡ PairT t2 t2'
+  | teq_SumT t1 t2 t1' t2' : t1 ≡ t2 -> t1' ≡ t2' -> SumT t1 t1' ≡ SumT t2 t2'
+  | teq_SumNT n f1 f2 : (∀ i, f1 i ≡ f2 i) -> SumNT n f1 ≡ SumNT n f2
+  | teq_FunT t1 t2 t1' t2' : t1 ≡ t2 -> t1' ≡ t2' -> FunT t1 t1' ≡ FunT t2 t2'
+  | teq_UFunT t1 t2 t1' t2' : t1 ≡ t2 -> t1' ≡ t2' -> UFunT t1 t1' ≡ UFunT t2 t2'
+  | teq_ChanT s1 s2 : s1 ≡ s2 -> ChanT s1 ≡ ChanT s2.
 Existing Instance type_equiv.
 
 Global Instance type_equivalence : Equivalence (≡@{type}).
 Proof.
-    split.
-    - cofix IH. intros []; constructor; done || apply session_type_reflexive, _.
-    - cofix IH. intros ??[]; constructor; done || by apply (session_type_symmetric _).
-    - cofix IH. intros ???[]; inversion_clear 1; constructor;
-      by etrans || by eapply (session_type_transitive _).
+  split.
+  - cofix IH. intros []; constructor; done || apply session_type_reflexive, _.
+  - cofix IH. intros ??[]; constructor; done || by apply (session_type_symmetric _).
+  - cofix IH. intros ???[]; try solve [inversion_clear 1; constructor;
+    (by etrans || by eapply (session_type_transitive _))].
+    intros Q. remember (SumNT n f2) as X.
+    inversion Q; simplify_eq. constructor.
+    intro. etrans; eauto.
 Qed.
 
 Canonical Structure typeO := discreteO type.
@@ -170,16 +179,18 @@ Notation session_typeO := (session_type'O typeO).
 Notation envT := (gmap string type).
 
 CoInductive unrestricted : type -> Prop :=
-    | Nat_unrestricted : unrestricted NatT
-    | Unit_unrestricted : unrestricted UnitT
-    | Void_unrestricted : unrestricted VoidT
-    | UFun_unrestricted t1 t2 : unrestricted (UFunT t1 t2)
-    | Pair_unrestricted t1 t2 :
-        unrestricted t1 -> unrestricted t2 ->
-        unrestricted (PairT t1 t2)
-    | Sum_unrestricted t1 t2 :
-        unrestricted t1 -> unrestricted t2 ->
-        unrestricted (SumT t1 t2).
+  | Nat_unrestricted : unrestricted NatT
+  | Unit_unrestricted : unrestricted UnitT
+  | Void_unrestricted : unrestricted VoidT
+  | UFun_unrestricted t1 t2 : unrestricted (UFunT t1 t2)
+  | Pair_unrestricted t1 t2 :
+    unrestricted t1 -> unrestricted t2 ->
+    unrestricted (PairT t1 t2)
+  | Sum_unrestricted t1 t2 :
+    unrestricted t1 -> unrestricted t2 ->
+    unrestricted (SumT t1 t2)
+  | SumN_unrestricted n f :
+    (∀ i, unrestricted (f i)) -> unrestricted (SumNT n f).
 
 Definition disj (Γ1 Γ2 : envT) : Prop :=
   ∀ i t1 t2, Γ1 !! i = Some t1 -> Γ2 !! i = Some t2 -> t1 ≡ t2 ∧ unrestricted t1.
@@ -204,102 +215,111 @@ Qed.
 
 Instance disj_union_Proper n : Proper ((≡) ==> (=) ==> (≡)) (disj_union n).
 Proof.
-    intros ??????.
-    split; subst; eauto using disj_union_Proper_impl.
-    symmetry in H. eauto using disj_union_Proper_impl.
+  intros ??????.
+  split; subst; eauto using disj_union_Proper_impl.
+  symmetry in H. eauto using disj_union_Proper_impl.
 Qed.
 
 Inductive typed : envT -> expr -> type -> Prop :=
-    | Unit_typed Γ :
-        Γunrestricted Γ ->
-        typed Γ (Val UnitV) UnitT
-    | Nat_typed : ∀ Γ n,
-        Γunrestricted Γ ->
-        typed Γ (Val (NatV n)) NatT
-    | Var_typed : ∀ Γ x t t',
-        Γ !! x = None ->
-        Γunrestricted Γ ->
-        t ≡ t' ->
-        typed (Γ ∪ {[ x := t ]}) (Var x) t'
-    | Pair_typed : ∀ Γ1 Γ2 e1 e2 t1 t2,
-        disj Γ1 Γ2 ->
-        typed Γ1 e1 t1 ->
-        typed Γ2 e2 t2 ->
-        typed (Γ1 ∪ Γ2) (Pair e1 e2) (PairT t1 t2)
-    | App_typed : ∀ Γ1 Γ2 e1 e2 t1 t2,
-        disj Γ1 Γ2 ->
-        typed Γ1 e1 (FunT t1 t2) ->
-        typed Γ2 e2 t1 ->
-        typed (Γ1 ∪ Γ2) (App e1 e2) t2
-    | UApp_typed : ∀ Γ1 Γ2 e1 e2 t1 t2,
-        disj Γ1 Γ2 ->
-        typed Γ1 e1 (UFunT t1 t2) ->
-        typed Γ2 e2 t1 ->
-        typed (Γ1 ∪ Γ2) (UApp e1 e2) t2
-    | Lam_typed : ∀ Γ x e t1 t2,
-        Γ !! x = None ->
-        typed (Γ ∪ {[ x := t1 ]}) e t2 ->
-        typed Γ (Lam x e) (FunT t1 t2)
-    | ULam_typed : ∀ Γ x e t1 t2,
-        Γ !! x = None ->
-        Γunrestricted Γ ->
-        typed (Γ ∪ {[ x := t1 ]}) e t2 ->
-        typed Γ (ULam x e) (UFunT t1 t2)
-    | Send_typed : ∀ Γ1 Γ2 e1 e2 t r p,
-        disj Γ1 Γ2 ->
-        typed Γ1 e1 (ChanT (SendT p t r)) ->
-        typed Γ2 e2 t ->
-        typed (Γ1 ∪ Γ2) (Send p e1 e2) (ChanT r)
-    | Recv_typed : ∀ Γ e t r p,
-        typed Γ e (ChanT (RecvT p t r)) ->
-        typed Γ (Recv p e) (PairT (ChanT r) t)
-    | Let_typed : ∀ Γ1 Γ2 e1 e2 t1 t2 x,
-        disj Γ1 Γ2 ->
-        Γ2 !! x = None ->
-        typed Γ1 e1 t1 ->
-        typed (Γ2 ∪ {[ x := t1 ]}) e2 t2 ->
-        typed (Γ1 ∪ Γ2) (Let x e1 e2) t2
-    | LetUnit_typed : ∀ Γ1 Γ2 e1 e2 t,
-        disj Γ1 Γ2 ->
-        typed Γ1 e1 UnitT ->
-        typed Γ2 e2 t ->
-        typed (Γ1 ∪ Γ2) (LetUnit e1 e2) t
-    | LetProd_typed : ∀ Γ1 Γ2 e1 e2 t11 t12 t2 x1 x2,
-        disj Γ1 Γ2 ->
-        x1 ≠ x2 ->
-        Γ2 !! x1 = None ->
-        Γ2 !! x2 = None ->
-        typed Γ1 e1 (PairT t11 t12) ->
-        typed (Γ2 ∪ {[ x1 := t11 ]} ∪ {[ x2 := t12 ]}) e2 t2 ->
-        typed (Γ1 ∪ Γ2) (LetProd x1 x2 e1 e2) t2
-    | MatchVoid_typed : ∀ Γ e t,
-        typed Γ e VoidT ->
-        typed Γ (MatchVoid e) t
-    | MatchSum_typed : ∀ Γ1 Γ2 e1 eL eR tL tR t x,
-        disj Γ1 Γ2 ->
-        Γ2 !! x = None ->
-        typed Γ1 e1 (SumT tL tR) ->
-        typed (Γ2 ∪ {[ x := tL ]}) eL t ->
-        typed (Γ2 ∪ {[ x := tR ]}) eR t ->
-        typed (Γ1 ∪ Γ2) (MatchSum e1 x eL eR) t
-    | If_typed : ∀ Γ1 Γ2 e1 e2 e3 t,
-        disj Γ1 Γ2 ->
-        typed Γ1 e1 NatT ->
-        typed Γ2 e2 t ->
-        typed Γ2 e3 t ->
-        typed (Γ1 ∪ Γ2) (If e1 e2 e3) t
-    | Spawn_typed : ∀ n Γ fΓ σs f,
-        consistent n σs ->
-        disj_union n Γ fΓ ->
-        (∀ p, typed (fΓ p) (f p) (FunT (ChanT (σs p)) UnitT)) ->
-        typed Γ (Spawn n f) UnitT
-    | Close_typed : ∀ Γ e,
-        typed Γ e (ChanT EndT) ->
-        typed Γ (Close e) UnitT
-    | Iso_typed : ∀ Γ t t' e,
-        t ≡ t' -> (* The ≡-relation is unfolding of recursive types *)
-        typed Γ e t ->
-        typed Γ e t'.
+  | Unit_typed Γ :
+    Γunrestricted Γ ->
+    typed Γ (Val UnitV) UnitT
+  | Nat_typed : ∀ Γ n,
+    Γunrestricted Γ ->
+    typed Γ (Val (NatV n)) NatT
+  | Var_typed : ∀ Γ x t t',
+    Γ !! x = None ->
+    Γunrestricted Γ ->
+    t ≡ t' ->
+    typed (Γ ∪ {[ x := t ]}) (Var x) t'
+  | Pair_typed : ∀ Γ1 Γ2 e1 e2 t1 t2,
+    disj Γ1 Γ2 ->
+    typed Γ1 e1 t1 ->
+    typed Γ2 e2 t2 ->
+    typed (Γ1 ∪ Γ2) (Pair e1 e2) (PairT t1 t2)
+  | App_typed : ∀ Γ1 Γ2 e1 e2 t1 t2,
+    disj Γ1 Γ2 ->
+    typed Γ1 e1 (FunT t1 t2) ->
+    typed Γ2 e2 t1 ->
+    typed (Γ1 ∪ Γ2) (App e1 e2) t2
+  | UApp_typed : ∀ Γ1 Γ2 e1 e2 t1 t2,
+    disj Γ1 Γ2 ->
+    typed Γ1 e1 (UFunT t1 t2) ->
+    typed Γ2 e2 t1 ->
+    typed (Γ1 ∪ Γ2) (UApp e1 e2) t2
+  | Lam_typed : ∀ Γ x e t1 t2,
+    Γ !! x = None ->
+    typed (Γ ∪ {[ x := t1 ]}) e t2 ->
+    typed Γ (Lam x e) (FunT t1 t2)
+  | ULam_typed : ∀ Γ x e t1 t2,
+    Γ !! x = None ->
+    Γunrestricted Γ ->
+    typed (Γ ∪ {[ x := t1 ]}) e t2 ->
+    typed Γ (ULam x e) (UFunT t1 t2)
+  | Send_typed : ∀ Γ1 Γ2 e1 e2 t r p,
+    disj Γ1 Γ2 ->
+    typed Γ1 e1 (ChanT (SendT p t r)) ->
+    typed Γ2 e2 t ->
+    typed (Γ1 ∪ Γ2) (Send p e1 e2) (ChanT r)
+  | Recv_typed : ∀ Γ e t r p,
+    typed Γ e (ChanT (RecvT p t r)) ->
+    typed Γ (Recv p e) (PairT (ChanT r) t)
+  | Let_typed : ∀ Γ1 Γ2 e1 e2 t1 t2 x,
+    disj Γ1 Γ2 ->
+    Γ2 !! x = None ->
+    typed Γ1 e1 t1 ->
+    typed (Γ2 ∪ {[ x := t1 ]}) e2 t2 ->
+    typed (Γ1 ∪ Γ2) (Let x e1 e2) t2
+  | LetUnit_typed : ∀ Γ1 Γ2 e1 e2 t,
+    disj Γ1 Γ2 ->
+    typed Γ1 e1 UnitT ->
+    typed Γ2 e2 t ->
+    typed (Γ1 ∪ Γ2) (LetUnit e1 e2) t
+  | LetProd_typed : ∀ Γ1 Γ2 e1 e2 t11 t12 t2 x1 x2,
+    disj Γ1 Γ2 ->
+    x1 ≠ x2 ->
+    Γ2 !! x1 = None ->
+    Γ2 !! x2 = None ->
+    typed Γ1 e1 (PairT t11 t12) ->
+    typed (Γ2 ∪ {[ x1 := t11 ]} ∪ {[ x2 := t12 ]}) e2 t2 ->
+    typed (Γ1 ∪ Γ2) (LetProd x1 x2 e1 e2) t2
+  | MatchVoid_typed : ∀ Γ e t,
+    typed Γ e VoidT ->
+    typed Γ (MatchVoid e) t
+  | MatchSum_typed : ∀ Γ1 Γ2 e1 eL eR tL tR t x,
+    disj Γ1 Γ2 ->
+    Γ2 !! x = None ->
+    typed Γ1 e1 (SumT tL tR) ->
+    typed (Γ2 ∪ {[ x := tL ]}) eL t ->
+    typed (Γ2 ∪ {[ x := tR ]}) eR t ->
+    typed (Γ1 ∪ Γ2) (MatchSum e1 x eL eR) t
+  | InjN_typed : ∀ Γ n f i e,
+    typed Γ e (f i) ->
+    typed Γ (InjN (fin_to_nat i) e) (SumNT n f)
+  | MatchSumN_typed : ∀ n Γ1 Γ2 Γ2' t f fc e,
+    disj Γ1 Γ2 ->
+    disj_union n Γ2 Γ2' ->
+    typed Γ1 e (SumNT n f) ->
+    (∀ i, typed (Γ2' i) (fc i) (FunT (f i) t)) ->
+    typed (Γ1 ∪ Γ2) (MatchSumN n e fc) t
+  | If_typed : ∀ Γ1 Γ2 e1 e2 e3 t,
+    disj Γ1 Γ2 ->
+    typed Γ1 e1 NatT ->
+    typed Γ2 e2 t ->
+    typed Γ2 e3 t ->
+    typed (Γ1 ∪ Γ2) (If e1 e2 e3) t
+  | Spawn_typed : ∀ n Γ fΓ σs f,
+    consistent n σs ->
+    disj_union n Γ fΓ ->
+    (∀ p, typed (fΓ p) (f p) (FunT (ChanT (σs p)) UnitT)) ->
+    typed Γ (Spawn n f) UnitT
+  | Close_typed : ∀ Γ e,
+    typed Γ e (ChanT EndT) ->
+    typed Γ (Close e) UnitT
+  | Iso_typed : ∀ Γ t t' e,
+    t ≡ t' -> (* The ≡-relation is unfolding of recursive types *)
+    typed Γ e t ->
+    typed Γ e t'.
 
 Fixpoint subst (x:string) (a:val) (e:expr) : expr :=
   match e with
@@ -316,125 +336,132 @@ Fixpoint subst (x:string) (a:val) (e:expr) : expr :=
   | Let x' e1 e2 => Let x' (subst x a e1) (if decide (x = x') then e2 else subst x a e2)
   | LetUnit e1 e2 => LetUnit (subst x a e1) (subst x a e2)
   | LetProd x' y' e1 e2 =>
-      LetProd x' y' (subst x a e1) (if decide (x = x' ∨ x = y') then e2 else subst x a e2)
+    LetProd x' y' (subst x a e1) (if decide (x = x' ∨ x = y') then e2 else subst x a e2)
   | MatchVoid e1 => MatchVoid (subst x a e1)
   | MatchSum e1 x' eL eR =>
-      MatchSum (subst x a e1) x'
-        (if decide (x = x') then eL else subst x a eL)
-        (if decide (x = x') then eR else subst x a eR)
+    MatchSum (subst x a e1) x'
+    (if decide (x = x') then eL else subst x a eL)
+    (if decide (x = x') then eR else subst x a eR)
+  | InjN n e => InjN n (subst x a e)
+  | MatchSumN n e f => MatchSumN n (subst x a e) (λ i, subst x a (f i))
   | If e1 e2 e3 => If (subst x a e1) (subst x a e2) (subst x a e3)
   | Spawn ps f => Spawn ps (λ p, subst x a (f p))
   | Close e1 => Close (subst x a e1)
   end.
 
 Inductive pure_step : expr -> expr -> Prop :=
-    | Pair_step : ∀ v1 v2,
-        pure_step (Pair (Val v1) (Val v2)) (Val (PairV v1 v2))
-    | Inj_step : ∀ v1 b,
-        pure_step (Inj b (Val v1)) (Val (InjV b v1))
-    | App_step : ∀ x e a,
-        pure_step (App (Val (FunV x e)) (Val a)) (subst x a e)
-    | UApp_step : ∀ x e a,
-        pure_step (UApp (Val (UFunV x e)) (Val a)) (subst x a e)
-    | Lam_step : ∀ x e,
-        pure_step (Lam x e) (Val (FunV x e))
-    | ULam_step : ∀ x e,
-        pure_step (ULam x e) (Val (UFunV x e))
-    | If_step1 : ∀ n e1 e2,
-        n ≠ 0 ->
-        pure_step (If (Val (NatV n)) e1 e2) e1
-    | If_step2 : ∀ e1 e2,
-        pure_step (If (Val (NatV 0)) e1 e2) e2
-    | MatchSum_step : ∀ x v eL eR b,
-        pure_step (MatchSum (Val (InjV b v)) x eL eR)
-            (if b then subst x v eL else subst x v eR)
-    | Let_step : ∀ x v e,
-        pure_step (Let x (Val v) e) (subst x v e)
-    | LetUnit_step : ∀ e,
-        pure_step (LetUnit (Val UnitV) e) e
-    | LetProd_step : ∀ x1 x2 v1 v2 e,
-        pure_step (LetProd x1 x2 (Val (PairV v1 v2)) e) (subst x1 v1 $ subst x2 v2 e).
+  | Pair_step : ∀ v1 v2,
+    pure_step (Pair (Val v1) (Val v2)) (Val (PairV v1 v2))
+  | Inj_step : ∀ v1 b,
+    pure_step (Inj b (Val v1)) (Val (InjV b v1))
+  | App_step : ∀ x e a,
+    pure_step (App (Val (FunV x e)) (Val a)) (subst x a e)
+  | UApp_step : ∀ x e a,
+    pure_step (UApp (Val (UFunV x e)) (Val a)) (subst x a e)
+  | Lam_step : ∀ x e,
+    pure_step (Lam x e) (Val (FunV x e))
+  | ULam_step : ∀ x e,
+    pure_step (ULam x e) (Val (UFunV x e))
+  | If_step1 : ∀ n e1 e2,
+    n ≠ 0 ->
+    pure_step (If (Val (NatV n)) e1 e2) e1
+  | If_step2 : ∀ e1 e2,
+    pure_step (If (Val (NatV 0)) e1 e2) e2
+  | MatchSum_step : ∀ x v eL eR b,
+    pure_step (MatchSum (Val (InjV b v)) x eL eR)
+      (if b then subst x v eL else subst x v eR)
+  | InjN_step : ∀ n v,
+    pure_step (InjN n (Val v)) (Val (InjNV n v))
+  | MatchSumN_step : ∀ n i v f,
+    pure_step (MatchSumN n (Val (InjNV (fin_to_nat i) v)) f) (App (f i) (Val v))
+  | Let_step : ∀ x v e,
+    pure_step (Let x (Val v) e) (subst x v e)
+  | LetUnit_step : ∀ e,
+    pure_step (LetUnit (Val UnitV) e) e
+  | LetProd_step : ∀ x1 x2 v1 v2 e,
+    pure_step (LetProd x1 x2 (Val (PairV v1 v2)) e) (subst x1 v1 $ subst x2 v2 e).
 
 Definition heap := gmap endpoint (gmap participant (list val)).
 
 Definition init_chan n : gmap participant (list val) :=
-    fin_gmap n (λ i, []).
+  fin_gmap n (λ i, []).
 Definition init_chans n : gmap participant (gmap participant (list val)) :=
-    fin_gmap n (λ i, init_chan n).
+  fin_gmap n (λ i, init_chan n).
 
 Definition init_threads (c : session) (n : nat) (fv : fin n -> val) : list expr :=
-    fin_list n (λ i, App (Val (fv i)) (Val (ChanV (c, fin_to_nat i)))).
+  fin_list n (λ i, App (Val (fv i)) (Val (ChanV (c, fin_to_nat i)))).
 
 Inductive head_step : expr -> heap -> expr -> heap -> list expr -> Prop :=
-    | Pure_step : ∀ e e' h,
-        pure_step e e' -> head_step e h e' h []
-    | Send_step : ∀ h c p q y, (* p is us, q is the one we send to *)
-                               (* send puts the value in the bufs of the other *)
-                               (* since we are participant p, we put it in that buffer *)
-        head_step (Send q (Val (ChanV (c,p))) (Val y)) h
-                  (Val (ChanV (c,p))) (alter (alter (λ buf, buf ++ [y]) p) (c,q) h) []
-        (* We could instead to the following:
-           (that would move some of the work from the preservation proof to the progress proof.) *)
-        (*
-        h !! (c,q) = Some bufs ->
-        bufs !! p = Some buf ->
-        head_step (Send q (Val (ChanV (c,p))) (Val y)) h
-                  (Val (ChanV (c,p))) (<[ (c,q) := <[ p := buf ++ [y] ]> bufs ]> h) []
-        *)
-    | Recv_step : ∀ h c p q y bufs buf, (* p is us, q is the one we recv from *)
-        h !! (c,p) = Some bufs -> (* recv takes the value out of its own bufs *)
-        bufs !! q = Some (y::buf) -> (* since the recv is from p, we take it out of that buffer *)
-        head_step (Recv q (Val (ChanV (c,p)))) h
-                  (Val (PairV (ChanV (c,p)) y)) (<[ (c,p) := <[ q := buf ]> bufs ]> h) []
-    | Close_step : ∀ c p h,
-        (* We can add these conditions: that would move some of the work from the
-           preservation proof to the progress proof. *)
-        (* h !! (c,p) = Some bufs -> *)
-        (* (∀ q, bufs !! q = Some []) -> *)
-        head_step (Close (Val (ChanV (c,p)))) h
-                  (Val UnitV) (delete (c,p) h) []
-    | Spawn_step : ∀ (h : heap) c n f fv,
-        (∀ p, h !! (c,p) = None) ->
-        (∀ p, f p = Val (fv p)) ->
-        head_step
-          (Spawn n f) h
-          (Val UnitV) (gmap_unslice (init_chans n) c ∪ h)
-          (init_threads c n fv).
+  | Pure_step : ∀ e e' h,
+    pure_step e e' -> head_step e h e' h []
+  | Send_step : ∀ h c p q y, (* p is us, q is the one we send to *)
+                 (* send puts the value in the bufs of the other *)
+                 (* since we are participant p, we put it in that buffer *)
+    head_step (Send q (Val (ChanV (c,p))) (Val y)) h
+          (Val (ChanV (c,p))) (alter (alter (λ buf, buf ++ [y]) p) (c,q) h) []
+    (* We could instead to the following:
+       (that would move some of the work from the preservation proof to the progress proof.) *)
+    (*
+    h !! (c,q) = Some bufs ->
+    bufs !! p = Some buf ->
+    head_step (Send q (Val (ChanV (c,p))) (Val y)) h
+          (Val (ChanV (c,p))) (<[ (c,q) := <[ p := buf ++ [y] ]> bufs ]> h) []
+    *)
+  | Recv_step : ∀ h c p q y bufs buf, (* p is us, q is the one we recv from *)
+    h !! (c,p) = Some bufs -> (* recv takes the value out of its own bufs *)
+    bufs !! q = Some (y::buf) -> (* since the recv is from p, we take it out of that buffer *)
+    head_step (Recv q (Val (ChanV (c,p)))) h
+          (Val (PairV (ChanV (c,p)) y)) (<[ (c,p) := <[ q := buf ]> bufs ]> h) []
+  | Close_step : ∀ c p h,
+    (* We can add these conditions: that would move some of the work from the
+       preservation proof to the progress proof. *)
+    (* h !! (c,p) = Some bufs -> *)
+    (* (∀ q, bufs !! q = Some []) -> *)
+    head_step (Close (Val (ChanV (c,p)))) h
+          (Val UnitV) (delete (c,p) h) []
+  | Spawn_step : ∀ (h : heap) c n f fv,
+    (∀ p, h !! (c,p) = None) ->
+    (∀ p, f p = Val (fv p)) ->
+    head_step
+      (Spawn n f) h
+      (Val UnitV) (gmap_unslice (init_chans n) c ∪ h)
+      (init_threads c n fv).
 
 Inductive ctx1 : (expr -> expr) -> Prop :=
-    | Ctx_App_l e : ctx1 (λ x, App x e)
-    | Ctx_App_r v : ctx1 (λ x, App (Val v) x)
-    | Ctx_Pair_l e : ctx1 (λ x, Pair x e)
-    | Ctx_Pair_r v : ctx1 (λ x, Pair (Val v) x)
-    | Ctx_Inj b : ctx1 (λ x, Inj b x)
-    | Ctx_UApp_l e : ctx1 (λ x, UApp x e)
-    | Ctx_UApp_r v : ctx1 (λ x, UApp (Val v) x)
-    | Ctx_Send_l p e : ctx1 (λ x, Send p x e)
-    | Ctx_Send_r p v : ctx1 (λ x, Send p (Val v) x)
-    | Ctx_Recv p : ctx1 (λ x, Recv p x)
-    | Ctx_Let s e : ctx1 (λ x, Let s x e)
-    | Ctx_LetUnit e : ctx1 (λ x, LetUnit x e)
-    | Ctx_LetProd s1 s2 e : ctx1 (λ x, LetProd s1 s2 x e)
-    | Ctx_MatchVoid : ctx1 (λ x, MatchVoid x)
-    | Ctx_MatchSum s e1 e2 : ctx1 (λ x, MatchSum x s e1 e2)
-    | Ctx_If e1 e2 : ctx1 (λ x, If x e1 e2)
-    | Ctx_Spawn n (f : fin n -> expr) (p : fin n) :
-        ctx1 (λ x, Spawn n (λ q, if decide (p = q) then x else f q))
-    | Ctx_Close : ctx1 (λ x, Close x).
+  | Ctx_App_l e : ctx1 (λ x, App x e)
+  | Ctx_App_r v : ctx1 (λ x, App (Val v) x)
+  | Ctx_Pair_l e : ctx1 (λ x, Pair x e)
+  | Ctx_Pair_r v : ctx1 (λ x, Pair (Val v) x)
+  | Ctx_Inj b : ctx1 (λ x, Inj b x)
+  | Ctx_UApp_l e : ctx1 (λ x, UApp x e)
+  | Ctx_UApp_r v : ctx1 (λ x, UApp (Val v) x)
+  | Ctx_Send_l p e : ctx1 (λ x, Send p x e)
+  | Ctx_Send_r p v : ctx1 (λ x, Send p (Val v) x)
+  | Ctx_Recv p : ctx1 (λ x, Recv p x)
+  | Ctx_Let s e : ctx1 (λ x, Let s x e)
+  | Ctx_LetUnit e : ctx1 (λ x, LetUnit x e)
+  | Ctx_LetProd s1 s2 e : ctx1 (λ x, LetProd s1 s2 x e)
+  | Ctx_MatchVoid : ctx1 (λ x, MatchVoid x)
+  | Ctx_MatchSum s e1 e2 : ctx1 (λ x, MatchSum x s e1 e2)
+  | Ctx_MatchSumN n (f : fin n -> expr) : ctx1 (λ x, MatchSumN n x f)
+  | Ctx_If e1 e2 : ctx1 (λ x, If x e1 e2)
+  | Ctx_Spawn n (f : fin n -> expr) (p : fin n) :
+    ctx1 (λ x, Spawn n (λ q, if decide (p = q) then x else f q))
+  | Ctx_Close : ctx1 (λ x, Close x).
 
 Inductive ctx : (expr -> expr) -> Prop :=
-    | Ctx_nil : ctx (λ x, x)
-    | Ctx_cons : ∀ k1 k2, ctx1 k1 -> ctx k2 -> ctx (λ x, (k1 (k2 x))).
+  | Ctx_nil : ctx (λ x, x)
+  | Ctx_cons : ∀ k1 k2, ctx1 k1 -> ctx k2 -> ctx (λ x, (k1 (k2 x))).
 
 Inductive ctx_step : expr -> heap -> expr -> heap -> list expr -> Prop :=
   | Ctx_step : ∀ k e h e' h' ts,
-      ctx k -> head_step e h e' h' ts -> ctx_step (k e) h (k e') h' ts.
+    ctx k -> head_step e h e' h' ts -> ctx_step (k e) h (k e') h' ts.
 
 Inductive stepi : nat -> list expr -> heap -> list expr -> heap -> Prop :=
   | Head_step : ∀ e e' h h' i ts es,
-      ctx_step e h e' h' ts ->
-      es !! i = Some e ->
-      stepi i es h (<[i := e']> es ++ ts) h'.
+    ctx_step e h e' h' ts ->
+    es !! i = Some e ->
+    stepi i es h (<[i := e']> es ++ ts) h'.
 
 Definition step es h es' h' := ∃ i, stepi i es h es' h'.
 
@@ -443,8 +470,8 @@ Definition can_stepi i es h := ∃ es' h', stepi i es h es' h'.
 (* Closure of the step relation; this is used in the theorem statement. *)
 Inductive steps : list expr -> heap -> list expr -> heap -> Prop :=
   | Trans_step : ∀ e1 e2 e3 s1 s2 s3,
-      step e1 s1 e2 s2 ->
-      steps e2 s2 e3 s3 ->
-      steps e1 s1 e3 s3
+    step e1 s1 e2 s2 ->
+    steps e2 s2 e3 s3 ->
+    steps e1 s1 e3 s3
   | Empty_step : ∀ e1 s1,
-      steps e1 s1 e1 s1.
+    steps e1 s1 e1 s1.
