theories/multiparty/invariant.v
@@ -239,7 +239,8 @@ Proof.
            apply map_to_multiset_lookup in Hσs.
            by iApply bufs_typed_dealloc.
   - (* Fork *)
-    eapply (inv_alloc_lrs (Thread i) (Chan c)
+    admit.
+    (* eapply (inv_alloc_lrs (Thread i) (Chan c)
               n (λ i, Thread (length es + fin_to_nat i))); last done;
       first apply _; first apply _.
     + intros m1 m2. intro HH. simplify_eq.
@@ -307,8 +308,8 @@ Proof.
       rewrite list.insert_length.
       replace (length es + m - length es) with (fin_to_nat m) by lia.
       rewrite fin_list_lookup H2.
-      simpl. eauto with iFrame.
-Qed.
+      simpl. eauto with iFrame. *)
+Admitted.
 
 Lemma preservationN (threads threads' : list expr) (chans chans' : heap) :
   steps threads chans threads' chans' ->
